Program-proofs/Exercises/2D-counting/prob12/sol12PCStyle.dfy
@@ -1,0 +1,54 @@
+/*  file: sol12PCStyle.dfy
+    author: David De Potter
+    description: extra practice in Dafny, 2D-counting, 
+    solution to prob12
+    This is exercise 9.14 from the PC reader
+    NOTE: This solution follows the PC-style proof method described
+    in the general note on proof styles (see the README in the 
+    Exercises folder)
+*/
+
+include "../../commonSupport.dfy"
+import opened CommonFunctions
+import opened MonotonicityProps
+
+ghost function F(h:(int,int) -> int, x:int, y:int, z:int, m:nat): int
+requires Ordered2DInt(h, Asc, Asc)
+requires 0 < m
+requires 0 <= x <= m && 0 <= y
+decreases m - x + y
+{
+  if x >= m || y <= 0 then z
+  else if h(x,y-1) < 0 
+       then F(h, x+1, y, minimum(z, abs(h(x,y-1))), m)
+       else F(h, x, y-1, minimum(z, abs(h(x,y-1))), m)
+}
+
+method problem12(h:(int,int) -> int, m:nat, n:nat)
+returns (z:int)
+requires Ordered2DInt(h, Asc, Asc)
+requires 0 < m && 0 < n
+ensures z == F(h,0,n,abs(h(0,0)),m)
+{
+  var x:int, y:int := 0, n;
+  z := abs(h(0,0));
+
+  while x < m && 0 < y
+  invariant 0 <= x <= m
+  invariant 0 <= y <= n
+  invariant F(h,x,y,z,m) == F(h,0,n,abs(h(0,0)),m)
+  decreases m - x + y
+  {
+    z := minimum(z, abs(h(x,y-1)));
+
+    if h(x,y-1) < 0
+    {
+      x := x + 1;
+    }
+
+    else
+    {
+      y := y - 1;
+    }
+  }
+}
